Lean4Lean/Theory/Typing/Env.lean
@@ -1,7 +1,6 @@
 import Lean4Lean.Theory.Typing.Basic
 import Lean4Lean.Theory.VDecl
 import Lean4Lean.Theory.Quot
-import Lean4Lean.Theory.Inductive
 
 namespace Lean4Lean
 
@@ -42,7 +41,7 @@ inductive VDecl.WF : VEnv → VDecl → VEnv → Prop where
     VDecl.WF env .quot env'
   | induct :
     decl.WF env →
-    env.addInduct decl = some env' →
+    env.addInduct' decl = some env' →
     VDecl.WF env (.induct decl) env'
 
 inductive VEnv.WF' : List VDecl → VEnv → Prop where
