Lean4Lean/Theory/Typing/InductiveLemmas.lean
@@ -6,5 +6,5 @@ namespace Lean4Lean
 namespace VEnv
 
 theorem addInduct_WF (henv : Ordered env) (hdecl : decl.WF env)
-    (henv' : addInduct env decl = some env') : Ordered env' :=
+    (henv' : addInduct' env decl = some env') : Ordered env' :=
   sorry
